skeleton + comments added

code/kyber2/impl/Impl.Kyber2.Indcpa.fst
@@ -27,8 +27,65 @@ open Spec.Kyber2.FunctionInstantiation
 open Spec.Kyber2.CBD
 open Spec.Kyber2.Poly
 
+open Impl.Kyber2.NumericTypes.MontgomeryInt16
+
 open FStar.Math.Lemmas
 
 module Seq = Lib.Sequence
+module Buf = Lib.Buffer
 
+let pklen:size_t = size Spec.Kyber2.Indcpa.pklen
+let sklen:size_t = size Spec.Kyber2.Indcpa.sklen
+let ulen = size Spec.Kyber2.Indcpa.ulen
+let vlen = size Spec.Kyber2.Indcpa.vlen
+let ciphertextlen:size_t = size Spec.Kyber2.Indcpa.ciphertextlen
 
+val encode:
+  l:size_t{(v l)*params_n <= max_size_t}
+  -> x:poly
+  -> e:lbuffer uint8 (l*! ((size params_n) >>. 3))
+  -> Stack unit
+    (requires fun h -> live h x /\ live h e /\ Buf.disjoint x e)
+    (ensures fun h0 _ h1 -> modifies1 e h0 h1 /\ h1.[|e|] == Spec.Kyber2.Indcpa.encode (v l) (to_spec_poly h0 x))
+
+val decode:
+  l:size_t{(v l)*params_n <= max_size_t}
+  -> e:lbuffer uint8 (l*! ((size params_n) >>. 3))
+  -> x:poly
+  -> Stack unit
+    (requires fun h -> live h x /\ live h e /\ Buf.disjoint x e)
+    (ensures fun h0 _ h1 -> modifies1 x h0 h1 /\ (to_spec_poly h1 x) == Spec.Kyber2.Indcpa.decode (v l) h0.[|e|])
+
+val keygen:
+  (coins:lbuffer uint8 32ul)
+  -> pk:lbuffer uint8 pklen
+  -> sk:lbuffer uint8 sklen
+  -> Stack bool
+  (requires fun h -> live h coins /\ live h pk /\ live h sk /\ Buf.disjoint coins pk /\ Buf.disjoint coins sk /\ BUf.disjoint pk sk)
+  (ensures fun h0 b h1 -> modifies2 pk sk h0 h1 match Spec.Kyber2.Indcpa.keygen h0.[|coins|] with
+    |None --> b == false
+    |Some (p,s) -> b == true /\ h1.[|pk|] == p /\ h2.[|sk|] == s)
+
+val enc:
+  pk:lbuffer uint8 pklen
+  -> msg:lbuffer uint8 32ul
+  -> msgcoins:lbuffer uint8 32ul
+  -> ciphertext:lbuffer uint8 ciphertextlen
+  -> Stack bool
+    (requires fun h -> live h pk /\ live h msg /\ live h msgcoins /\ live h ciphertext /\
+                    Buf.disjoint pk msg /\ Buf.disjoint pk msgcoins /\ Buf.disjoint pk ciphertext /\
+                    Buf.disjoint msg msgcoins /\ Buf.disjoint msg ciphertext /\
+                    Buf.disjoint msgcoins ciphertext)
+    (ensures fun h0 b h1 -> modifies1 ciphertext h0 h1 /\ match Spec.Kyber2.Indcpa.enc h0.[|pk|] h0.[|msg|] h0.[|msgcoins|] with
+      |None -> b == false
+      |Some c -> b == true /\ h1.[|ciphertext|] == c)
+
+assume val dec
+  sk:lbuffer uint8 sklen
+  -> ciphertext:lbuffer uint8 ciphertextlen
+  -> msg':lbuffer uint8 32ul
+  -> Stack unit
+    (requires fun h -> live h pk /\ live h msg /\ live h msgcoins /\ live h ciphertext /\
+                    Buf.disjoint sk ciphertext /\ Buf.disjoint sk msg' /\
+                    Buf.disjoint msg' ciphertext)
+    (ensures fun h0 b h1 -> modifies1 msg' h0 h1 /\ h1.[|msg'|] == Spec.Kyber2.Indcpa.dec h0.[|sk|] h0.[|c|])
