code/kyber2/impl/Impl.Kyber2.NumericTypes.MontgomeryInt16.fst
@@ -21,12 +21,13 @@ module Buf = Lib.Buffer
 module MGroup = Impl.Kyber2.GroupMontgomery
 module Group = Impl.Kyber2.Group
 
-type num = int16
+type num = x:int16{sint_v x > - pow2 15}
 type poly = lbuffer num (size params_n)
 type vec = lbuffer num ((size params_k)*!(size params_n))
 type matrix = lbuffer num ((size params_k)*!(size params_k)*!(size params_n))
 
 #reset-options "--z3rlimit 500 --max_fuel 2 --max_ifuel 2"
+let to_spec_poly (h:mem) (p:poly) : Ghost (Spec.Kyber2.NumericTypes.poly) (requires T) (ensures fun p' -> p' == Seq.map MGroup.int16_to_t h.[|p|]) = Seq.map MGroup.int16_to_t h.[|p|]
 
 let to_spec_vec (h:mem) (v:vec) : Ghost (Spec.Kyber2.NumericTypes.vec) (requires True) (ensures fun v' -> forall (i:size_nat{i<params_k}). Spec.Kyber2.NumericTypes.index_vec v' i == Seq.map MGroup.int16_to_t h.[|gsub v (size i *! size params_n) (size params_n)|]) =
   let vec_aux (j:size_nat{j<=params_k}) : Type0 = v':Spec.Kyber2.NumericTypes.vec{forall (k:size_nat{k < j}). Spec.Kyber2.NumericTypes.index_vec v' k == Seq.map MGroup.int16_to_t h.[|gsub v (size k *! size params_n) (size params_n)|]} in
@@ -43,6 +44,10 @@ let to_spec_matrix (h:mem) (m:matrix) : Ghost (Spec.Kyber2.NumericTypes.matrix) 
     let v = to_spec_vec h (gsub m (size j *! size params_k *! size params_n) (size params_k *! size params_n)) in
     aux (j+1) (Spec.Kyber2.NumericTypes.upd_line acc j v) end
   in aux 0 (Spec.Kyber2.NumericTypes.new_matrix ())
+
+let to_spec_poly_lemma (h1 h2:mem) (p1 p2:vec) : Lemma (requires h1.[|p1|] == h2.[|p2|])
+  (ensures to_spec_poly h1 p1 == to_spec_poly h2 p2) =
+  eq_intro (to_spec_poly h1 v1) (to_spec_poly h2 v2)
 
 let to_spec_vec_lemma (h1 h2:mem) (v1 v2:vec) : Lemma (requires h1.[|v1|] == h2.[|v2|])
   (ensures to_spec_vec h1 v1 == to_spec_vec h2 v2) =
@@ -70,8 +75,8 @@ let to_spec_matrix_lemma (h1 h2:mem) (m1 m2:matrix) : Lemma (requires h1.[|m1|] 
 
 let new_poly () : StackInline (poly) (requires fun h0 -> True) (ensures fun h0 p h1 -> live h1 p /\ stack_allocated p h0 h1 (Seq.create params_n MGroup.zero_m) /\ Seq.map MGroup.int16_to_t h1.[|p|] == Spec.Kyber2.NumericTypes.new_poly ()) =
   assert_norm (MGroup.int16_to_t MGroup.zero_m == Group.zero_t);
-  eq_intro (Seq.map MGroup.int16_to_t (Seq.create params_n MGroup.zero_m)) (Spec.Kyber2.NumericTypes.new_poly ());
-  create (size params_n) (MGroup.zero_m)
+  eq_intro (Seq.map MGroup.int16_to_t (Seq.create #num params_n MGroup.zero_m)) (Spec.Kyber2.NumericTypes.new_poly ());
+  create (size params_n) MGroup.zero_m
 
 let new_vec () : StackInline (vec) (requires fun h0 -> True) (ensures fun h0 v h1 -> live h1 v /\ to_spec_vec h1 v == Spec.Kyber2.NumericTypes.new_vec ()) =
   assert_norm (MGroup.int16_to_t MGroup.zero_m == Group.zero_t);
@@ -107,16 +112,14 @@ let new_matrix () : StackInline (matrix) (requires fun h0 -> True) (ensures fun 
 #reset-options "--z3rlimit 1000 --max_fuel 2 --max_ifuel 2"
 
 val get_index_vec:
-  //#len:size_t
   (v:vec)
-  //-> (buf:lbuffer Group.t len)
   -> (i:size_t{Lib.IntTypes.v i < params_k})
   -> Stack (poly)
-    (requires fun h0 -> live h0 v)// /\ live h0 buf /\ Buf.disjoint v buf)
-    (ensures fun h0 p h1 -> h0 == h1 /\(* Buf.disjoint p buf /\*) p == gsub v (i*!(size params_n)) (size params_n) /\ Seq.map MGroup.int16_to_t h1.[|p|] == Spec.Kyber2.NumericTypes.index_vec (to_spec_vec h0 v) (Lib.IntTypes.v i))
+    (requires fun h0 -> live h0 v)
+    (ensures fun h0 p h1 -> h0 == h1 /\ p == gsub v (i*!(size params_n)) (size params_n) /\ Seq.map MGroup.int16_to_t h1.[|p|] == Spec.Kyber2.NumericTypes.index_vec (to_spec_vec h0 v) (Lib.IntTypes.v i))
 
 let get_index_vec v i = // #len v buf i =
-  Buf.sub #_ #int16 #(size params_k *! size params_n) v (i*!(size params_n)) (size params_n)
+  Buf.sub #_ #num #(size params_k *! size params_n) v (i*!(size params_n)) (size params_n)
 
 val get_index_vec_lemma:
   h0:mem
@@ -156,7 +159,7 @@ val get_line:
     (ensures fun h0 v' h1 -> h0 == h1 /\ v' == gsub m (i *! size params_k *! size params_n) (size params_k *! size params_n) /\ to_spec_vec h1 v' == Spec.Kyber2.NumericTypes.get_line (to_spec_matrix h0 m) (v i))
 
 let get_line m i =
-  Buf.sub #_ #int16 #(size params_k *! size params_k *! size params_n) m (i *! size params_k *! size params_n) (size params_k *! size params_n)
+  Buf.sub #_ #num #(size params_k *! size params_k *! size params_n) m (i *! size params_k *! size params_n) (size params_k *! size params_n)
 
 val get_line_lemma:
   h0:mem
@@ -213,7 +216,7 @@ let get_element m i j =
   as_seq_gsub h (gsub m (i *! size params_k *! size params_n) (size params_k *! size params_n)) (j *! size params_n) (size params_n);
   as_seq_gsub h m (((i *! size params_k) +! j) *! size params_n) (size params_n);
   eq_intro h.[|gsub (gsub m (i *! size params_k *! size params_n) (size params_k *! size params_n)) (j *! size params_n) (size params_n)|] h.[|gsub m (((i *! size params_k) +! j) *! size params_n) (size params_n)|];
-  Buf.sub #_ #int16 #(size params_k *! size params_k *! size params_n) m (((i*!size params_k) +! j) *! (size params_n)) (size params_n)
+  Buf.sub #_ #num #(size params_k *! size params_k *! size params_n) m (((i*!size params_k) +! j) *! (size params_n)) (size params_n)
 
 val get_element_lemma:
   h0:mem
@@ -448,3 +451,168 @@ let gen_matrix m spec_f impl_f =
   let h_end = ST.get () in
   to_spec_matrix_lemma h1 h_end m m;
   b
+
+#reset-options "--z3rlimit 400 --max_fuel 1 --max_ifuel 1 --print_universes"
+
+let lemma_test #a #n (x:lseq a n) : Lemma (of_list (to_list x) == x) =
+  FStar.Seq.Properties.lemma_seq_list_bij x
+
+noextract
+assume val zetas_list : x:(list MGroup.montgomery_t){List.length x = 128 /\ pow2 7 = 128 /\ (forall (k:size_nat{k<128}). MGroup.to_t (FStar.List.Tot.index x k) == Lib.Arithmetic.Ring.exp #Group.t #Spec.Kyber2.Ring.ring_t (Spec.Kyber2.Group.mk_t params_zeta) (Lib.Arithmetic.Sums.br 7 k))}
+
+noextract
+let zetas_seq : x:(lseq MGroup.montgomery_t 128){pow2 7 = 128 /\ (forall (k:size_nat{k<128}). MGroup.to_t x.[k] == Lib.Arithmetic.Ring.exp #Group.t #Spec.Kyber2.Ring.ring_t (Spec.Kyber2.Group.mk_t params_zeta) (Lib.Arithmetic.Sums.br 7 k))} = of_list zetas_list
+
+#reset-options "--z3rlimit 400 --max_fuel 2 --max_ifuel 1 --print_universes"
+
+let zetas : x:(ilbuffer MGroup.montgomery_t (size 128)){Buf.witnessed x zetas_seq /\ Buf.recallable x}
+=
+ Buf.createL_global zetas_list
+
+let lemma_mod (j:size_t{v j < params_n / 4}) : Lemma ((4*(v j)) % 2 = 0 /\ (4*(v j)+1) % 2 = 1 /\ (4*(v j)+2) % 2 = 0 /\ (4*(v j)+3) % 2 = 1 /\ 4*(v j)+3 < params_n /\ (4*(v j)) / 2 = 2*(v j) /\ (4*(v j)+2) / 2 = 2*(v j)+1 /\ 4*(v j) = (4*(v j)+1)-1 /\ 4*(v j)+2 = (4*(v j)+3) - 1) =
+  FStar.Math.Lemmas.paren_mul_right 2 2 (v j);
+  assert(4*(v j) = 2*(2*v j));
+  FStar.Math.Lemmas.swap_mul 2 (2*(v j));
+  FStar.Math.Lemmas.division_definition (4*(v j)) 2 (2*(v j));
+  FStar.Math.Lemmas.euclidean_division_definition (4*(v j)) 2;
+  assert((4*(v j))/2 = 2*(v j));
+  assert ((4*(v j)) % 2 = 0);
+  FStar.Math.Lemmas.modulo_distributivity (4 * (v j)) 1 2;
+  FStar.Math.Lemmas.modulo_distributivity (4 * (v j)) 2 2;
+  FStar.Math.Lemmas.modulo_distributivity (4 * (v j)) 3 2;
+  FStar.Math.Lemmas.modulo_distributivity 0 1 2;
+  FStar.Math.Lemmas.modulo_distributivity 0 2 2;
+  FStar.Math.Lemmas.modulo_distributivity 0 3 2;
+  FStar.Math.Lemmas.lemma_mod_twice 1 2;
+  FStar.Math.Lemmas.lemma_mod_twice 2 2;
+  FStar.Math.Lemmas.lemma_mod_twice 3 2;
+  assert ((4*(v j)+1) % 2 = 1);
+  assert ((4*(v j)+2) % 2 = 0);
+  assert ((4*(v j)+3) % 2 = 1);
+  FStar.Math.Lemmas.lemma_div_plus (4*(v j)) 1 2
+
+inline_for_extraction noextract
+val poly_mul_inner_odd:
+  p1:poly
+  -> p2:poly
+  -> output:poly
+  -> j:size_t{v j < params_n / 4}
+  -> Stack unit
+    (requires fun h -> live h p1 /\ live h p2 /\ live h output /\ Buf.disjoint p1 output /\ Buf.disjoint p2 output
+                    /\ (forall (k:nat{k<params_n}). v h.[|p1|].[k] <= params_q /\ v h.[|p1|].[k] >= - params_q) /\ (forall (k:nat{k<4*v j}). v h.[|output|].[k] <= 2 * params_q /\ v h.[|output|].[k] >= -2 * params_q /\ MGroup.int16_to_t h.[|output|].[k] == (Lib.Poly.NTT2.lib_ntt_mul #Group.t #Spec.Kyber2.Ring.ring_t #params_n 7 (Spec.Kyber2.Group.mk_t params_zeta) (Seq.map MGroup.int16_to_t h.[|p1|]) (Seq.map MGroup.int16_to_t h.[|p2|])).[k]))
+    (ensures fun h0 _ h1 -> live h1 p1 /\ live h1 p2 /\ live h1 output /\ Buf.disjoint p1 output /\ Buf.disjoint p2 output
+                       /\ modifies1 output h0 h1 /\ v h1.[|output|].[4*(v j)+1] <= 2 * params_q /\ v h1.[|output|].[4*(v j)+1] >= -2 * params_q /\ v h1.[|output|].[4*(v j)+3] <= 2 * params_q /\ v h1.[|output|].[4*(v j)+3] >= -2 * params_q /\ MGroup.int16_to_t h1.[|output|].[4*(v j)+1] == (Lib.Poly.NTT2.lib_ntt_mul #Group.t #Spec.Kyber2.Ring.ring_t #params_n 7 (Spec.Kyber2.Group.mk_t params_zeta) (Seq.map MGroup.int16_to_t h1.[|p1|]) (Seq.map MGroup.int16_to_t h1.[|p2|])).[4*(v j)+1] /\ MGroup.int16_to_t h1.[|output|].[4*(v j)+3] == (Lib.Poly.NTT2.lib_ntt_mul #Group.t #Spec.Kyber2.Ring.ring_t #params_n 7 (Spec.Kyber2.Group.mk_t params_zeta) (Seq.map MGroup.int16_to_t h1.[|p1|]) (Seq.map MGroup.int16_to_t h1.[|p2|])).[4*(v j)+3] /\ (forall (k:nat{k<4*v j}). v h1.[|output|].[k] <= 2 * params_q /\ v h1.[|output|].[k] >= -2 * params_q /\ MGroup.int16_to_t h1.[|output|].[k] == (Lib.Poly.NTT2.lib_ntt_mul #Group.t #Spec.Kyber2.Ring.ring_t #params_n 7 (Spec.Kyber2.Group.mk_t params_zeta) (Seq.map MGroup.int16_to_t h1.[|p1|]) (Seq.map MGroup.int16_to_t h1.[|p2|])).[k]))
+
+let poly_mul_inner_odd p1 p2 output j =
+  let h0 = ST.get () in
+  assert(4*(v j) +3 < params_n);
+  assert(v h0.[|p1|].[4*(v j)] <= params_q);
+  assert(v h0.[|p1|].[4*(v j)+1] <= params_q);
+  assert(v h0.[|p1|].[4*(v j)+2] <= params_q);
+  assert(v h0.[|p1|].[4*(v j)+3] <= params_q);
+  let f3 = MGroup.mul_m_int16 p2.((size 4)*!j) p1.(((size 4)*!j)+!1ul) in
+  let f7 = MGroup.mul_m_int16 p2.(((size 4)*!j) +! 2ul) p1.(((size 4)*!j)+!3ul) in
+  Spec.Kyber2.Ring.lemma_mul_swap_t (MGroup.int16_to_t h0.[|p2|].[4*(v j)]) (MGroup.int16_to_t h0.[|p1|].[4*(v j)+1]);
+  assert(MGroup.to_t f3 == Group.mul_t (MGroup.int16_to_t h0.[|p1|].[4*(v j)+1]) (MGroup.int16_to_t h0.[|p2|].[4*(v j)]));
+  output.(((size 4)*!j)+!1ul) <- f3 +! (MGroup.mul_m_int16 p2.(((size 4)*!j)+!1ul) p1.((size 4)*!j));
+  Spec.Kyber2.Ring.lemma_mul_swap_t (MGroup.int16_to_t h0.[|p2|].[4*(v j)+2]) (MGroup.int16_to_t h0.[|p1|].[4*(v j)+3]);
+  assert(MGroup.to_t f7 == Group.mul_t (MGroup.int16_to_t h0.[|p1|].[4*(v j)+3]) (MGroup.int16_to_t h0.[|p2|].[4*(v j)+2]));
+  output.(((size 4)*!j)+!3ul) <- f7 +! (MGroup.mul_m_int16 p2.(((size 4)*!j)+!3ul) p1.(((size 4)*!j)+!2ul));
+  let h_0 = ST.get () in
+  Spec.Kyber2.Ring.lemma_mul_swap_t (MGroup.int16_to_t h0.[|p2|].[4*(v j)+1]) (MGroup.int16_to_t h0.[|p1|].[4*(v j)]);
+  Spec.Kyber2.Ring.lemma_mul_swap_t (MGroup.int16_to_t h0.[|p2|].[4*(v j)+3]) (MGroup.int16_to_t h0.[|p1|].[4*(v j)+2]);
+  MGroup.plus_lemma_int16_2 f3 (MGroup.mul_m_int16 h0.[|p2|].[4*(v j)+1] h0.[|p1|].[4*(v j)]) (h_0.[|output|].[4*(v j) + 1]);
+  MGroup.plus_lemma_int16_2 f7 (MGroup.mul_m_int16 h0.[|p2|].[4*(v j)+3] h0.[|p1|].[4*(v j)+2]) (h_0.[|output|].[4*(v j) + 3]);
+  assert_norm(pow2 7 = params_n / 2);
+  lemma_mod j;
+  Lib.Poly.NTT2.lib_ntt_mul_odd_lemma_instantiate 7 (Spec.Kyber2.Group.mk_t params_zeta) (Seq.map MGroup.int16_to_t h0.[|p1|]) (Seq.map MGroup.int16_to_t h0.[|p2|]) (Lib.Poly.NTT2.lib_ntt_mul #Group.t #Spec.Kyber2.Ring.ring_t #params_n 7 (Spec.Kyber2.Group.mk_t params_zeta) (Seq.map MGroup.int16_to_t h0.[|p1|]) (Seq.map MGroup.int16_to_t h0.[|p2|])) (4*(v j)+1);
+  Lib.Poly.NTT2.lib_ntt_mul_odd_lemma_instantiate 7 (Spec.Kyber2.Group.mk_t params_zeta) (Seq.map MGroup.int16_to_t h0.[|p1|]) (Seq.map MGroup.int16_to_t h0.[|p2|]) (Lib.Poly.NTT2.lib_ntt_mul #Group.t #Spec.Kyber2.Ring.ring_t #params_n 7 (Spec.Kyber2.Group.mk_t params_zeta) (Seq.map MGroup.int16_to_t h0.[|p1|]) (Seq.map MGroup.int16_to_t h0.[|p2|])) (4*(v j)+3);
+  assert(MGroup.int16_to_t h_0.[|output|].[4*(v j) + 1] == Group.plus_t (Group.mul_t (MGroup.int16_to_t h0.[|p1|].[4*(v j)+1]) (MGroup.int16_to_t h0.[|p2|].[4*(v j)])) (Group.mul_t (MGroup.int16_to_t h0.[|p1|].[4*(v j)]) (MGroup.int16_to_t h0.[|p2|].[4*(v j)+1])));
+  assert((Seq.map MGroup.int16_to_t h0.[|p1|]).[4*(v j)] == MGroup.int16_to_t h0.[|p1|].[4*(v j)]);
+  assert((Seq.map MGroup.int16_to_t h0.[|p1|]).[4*(v j)+1] == MGroup.int16_to_t h0.[|p1|].[4*(v j)+1]);
+  assert((Seq.map MGroup.int16_to_t h0.[|p2|]).[4*(v j)] == MGroup.int16_to_t h0.[|p2|].[4*(v j)]);
+  assert((Seq.map MGroup.int16_to_t h0.[|p2|]).[4*(v j)+1] == MGroup.int16_to_t h0.[|p2|].[4*(v j)+1]);
+  assert (MGroup.int16_to_t h_0.[|output|].[4*(v j) + 1] == (Lib.Poly.NTT2.lib_ntt_mul #Group.t #Spec.Kyber2.Ring.ring_t #params_n 7 (Spec.Kyber2.Group.mk_t params_zeta) (Seq.map MGroup.int16_to_t h0.[|p1|]) (Seq.map MGroup.int16_to_t h0.[|p2|])).[4*(v j)+1]);
+  assert(MGroup.int16_to_t h_0.[|output|].[4*(v j) + 3] == Group.plus_t (Group.mul_t (MGroup.int16_to_t h0.[|p1|].[4*(v j)+3]) (MGroup.int16_to_t h0.[|p2|].[4*(v j)+2])) (Group.mul_t (MGroup.int16_to_t h0.[|p1|].[4*(v j)+2]) (MGroup.int16_to_t h0.[|p2|].[4*(v j)+3])));
+  assert((Seq.map MGroup.int16_to_t h0.[|p1|]).[4*(v j)+2] == MGroup.int16_to_t h0.[|p1|].[4*(v j)+2]);
+  assert((Seq.map MGroup.int16_to_t h0.[|p1|]).[4*(v j)+3] == MGroup.int16_to_t h0.[|p1|].[4*(v j)+3]);
+  assert((Seq.map MGroup.int16_to_t h0.[|p2|]).[4*(v j)+2] == MGroup.int16_to_t h0.[|p2|].[4*(v j)+2]);
+  assert((Seq.map MGroup.int16_to_t h0.[|p2|]).[4*(v j)+3] == MGroup.int16_to_t h0.[|p2|].[4*(v j)+3]);
+  assert (MGroup.int16_to_t h_0.[|output|].[4*(v j) + 3] == (Lib.Poly.NTT2.lib_ntt_mul #Group.t #Spec.Kyber2.Ring.ring_t #params_n 7 (Spec.Kyber2.Group.mk_t params_zeta) (Seq.map MGroup.int16_to_t h0.[|p1|]) (Seq.map MGroup.int16_to_t h0.[|p2|])).[4*(v j)+3])
+
+val poly_mul_inner:
+  p1:poly
+  -> p2:poly
+  -> output:poly
+  -> j:size_t{v j < params_n / 4}
+  -> Stack unit
+    (requires fun h -> live h p1 /\ live h p2 /\ live h output /\ Buf.disjoint p1 output /\ Buf.disjoint p2 output
+                    /\ (forall (k:nat{k<params_n}). v h.[|p1|].[k] <= params_q /\ v h.[|p1|].[k] >= - params_q) /\ (forall (k:nat{k<4*v j}). v h.[|output|].[k] <= 2 * params_q /\ v h.[|output|].[k] >= -2 * params_q /\ MGroup.int16_to_t h.[|output|].[k] == (Lib.Poly.NTT2.lib_ntt_mul #Group.t #Spec.Kyber2.Ring.ring_t #params_n 7 (Spec.Kyber2.Group.mk_t params_zeta) (Seq.map MGroup.int16_to_t h.[|p1|]) (Seq.map MGroup.int16_to_t h.[|p2|])).[k]))
+    (ensures fun h0 _ h1 -> live h1 p1 /\ live h1 p2 /\ live h1 output /\ Buf.disjoint p1 output /\ Buf.disjoint p2 output
+                       /\ modifies1 output h0 h1 /\ (forall (k:nat{k<4*(v j+1)}). v h1.[|output|].[k] <= 2 * params_q /\ v h1.[|output|].[k] >= -2 * params_q /\ MGroup.int16_to_t h1.[|output|].[k] == (Lib.Poly.NTT2.lib_ntt_mul #Group.t #Spec.Kyber2.Ring.ring_t #params_n 7 (Spec.Kyber2.Group.mk_t params_zeta) (Seq.map MGroup.int16_to_t h1.[|p1|]) (Seq.map MGroup.int16_to_t h1.[|p2|])).[k]))
+
+#reset-options "--z3rlimit 1000 --max_fuel 1 --max_ifuel 1 --print_universes"
+
+let poly_mul_inner p1 p2 output j =
+  let h0 = ST.get () in
+  poly_mul_inner_odd p1 p2 output j;
+  let h_0 = ST.get () in
+  assert(4*(v j) +3 < params_n);
+  assert(v h0.[|p1|].[4*(v j)] <= params_q);
+  assert(v h0.[|p1|].[4*(v j)+1] <= params_q);
+  assert(v h0.[|p1|].[4*(v j)+2] <= params_q);
+  assert(v h0.[|p1|].[4*(v j)+3] <= params_q);
+  assert (MGroup.int16_to_t h_0.[|output|].[4*(v j) + 1] == (Lib.Poly.NTT2.lib_ntt_mul #Group.t #Spec.Kyber2.Ring.ring_t #params_n 7 (Spec.Kyber2.Group.mk_t params_zeta) (Seq.map MGroup.int16_to_t h0.[|p1|]) (Seq.map MGroup.int16_to_t h0.[|p2|])).[4*(v j)+1]);
+  assert (MGroup.int16_to_t h_0.[|output|].[4*(v j) + 3] == (Lib.Poly.NTT2.lib_ntt_mul #Group.t #Spec.Kyber2.Ring.ring_t #params_n 7 (Spec.Kyber2.Group.mk_t params_zeta) (Seq.map MGroup.int16_to_t h0.[|p1|]) (Seq.map MGroup.int16_to_t h0.[|p2|])).[4*(v j)+3]);
+  let f1 = MGroup.mul_m_int16 p2.((size 4)*!j) p1.((size 4)*!j) in
+  Spec.Kyber2.Ring.lemma_mul_swap_t (MGroup.int16_to_t h0.[|p2|].[4*(v j)]) (MGroup.int16_to_t h0.[|p1|].[4*(v j)]);
+  assert(MGroup.to_t f1 == Group.mul_t (MGroup.int16_to_t h0.[|p1|].[4*(v j)]) (MGroup.int16_to_t h0.[|p2|].[4*(v j)]));
+  let f5 = MGroup.mul_m_int16 p2.(((size 4)*!j)+!2ul) p1.(((size 4)*!j)+!2ul) in
+  Spec.Kyber2.Ring.lemma_mul_swap_t (MGroup.int16_to_t h0.[|p2|].[4*(v j)+2]) (MGroup.int16_to_t h0.[|p1|].[4*(v j)+2]);
+  assert(MGroup.to_t f5 == Group.mul_t (MGroup.int16_to_t h0.[|p1|].[4*(v j)+2]) (MGroup.int16_to_t h0.[|p2|].[4*(v j)+2]));
+  assert_norm(params_n / 2 = 128 /\ params_n / 4 = pow2 6 /\ params_n / 2 = pow2 7);
+  Buf.recall_contents zetas zetas_seq;
+  assert_norm(params_n / 4 = pow2 6 /\ pow2 6 = 64);
+  assert_norm(v j < pow2 6);
+  assert_norm(pow2 7 = 128);
+  FStar.Math.Lemmas.pow2_double_sum 6;
+  let zeta = zetas.(j+!64ul) in
+  FStar.Math.Lemmas.division_definition (2*(v j)) 2 (v j);
+  FStar.Math.Lemmas.euclidean_division_definition (2*(v j)) 2;
+  assert((2*(v j)) % 2 = 0);
+  Lib.Arithmetic.Sums.br_lemma_n2_2 6 (2*(v j));
+  FStar.Math.Lemmas.pow2_double_sum 6;
+  FStar.Math.Lemmas.pow2_double_mult 6;
+  assert(Lib.Arithmetic.Sums.br 7 (2*(v j)) < pow2 6);
+  assert(Lib.Arithmetic.Sums.br 7 (2*(v j) + 1) == Lib.Arithmetic.Sums.br 7 (2*(v j)) + pow2 6);
+  FStar.Math.Lemmas.distributivity_add_right 2 (Lib.Arithmetic.Sums.br 7 (2*(v j))) (pow2 6);
+  FStar.Math.Lemmas.lemma_mult_le_left 2 (Lib.Arithmetic.Sums.br 7 (2*(v j))) (pow2 6 - 1);
+  FStar.Math.Lemmas.modulo_lemma (2*(Lib.Arithmetic.Sums.br 7 (2*(v j)))) (pow2 7);
+  Lib.Arithmetic.Sums.br_lemma_mul 7 (v j);
+  Lib.Arithmetic.Sums.br_lemma_n2_1 6 (v j);
+  assert(Lib.Arithmetic.Sums.br 7 (v j + 64) = 2*(Lib.Arithmetic.Sums.br 7 (2*(v j))) + 1);
+  assert(Lib.Arithmetic.Sums.br 7 (v j + 64) + 128 = 2*(Lib.Arithmetic.Sums.br 7 (2*(v j) + 1)) + 1); admit()
+  //let zeta = zetas.(j +! 64ul) in
+  assert(MGroup.to_t zetas_seq.[v j + 64] == Lib.Arithmetic.Ring.exp #Group.t #Spec.Kyber2.Ring.ring_t (Spec.Kyber2.Group.mk_t params_zeta) (2*(Lib.Arithmetic.Sums.br 7 (2*(v j))) +1)); admit()
+  Lib.Arithmetic.Ring.lemma_exp_morphism (Spec.Kyber2.Group.mk_t params_zeta) (Lib.Arithmetic.Sums.br 7 (v j + 64)) 128;
+  Spec.Kyber2.NTT.exp_correspondancy (Spec.Kyber2.Group.mk_t params_zeta) 128;
+  assert_norm (Lib.ModularArithmetic.modular_exp #params_q params_zeta 128 == (-1) % params_q);
+  let f2 = MGroup.mul_m_int16 p1.(((size 4) *! j) +! 1ul) (MGroup.mul_m_int16 p2.(((size 4) *!j) +! 1ul) zeta) in
+  Spec.Kyber2.Group.lemma_mul_assoc_t (MGroup.int16_to_t h0.[|p1|].[4*(v j)+1]) (MGroup.int16_to_t h0.[|p2|].[4*(v j)+1]) (MGroup.to_t zeta);
+  assert(MGroup.int16_to_t f2 == Group.mul_t (Group.mul_t (MGroup.int16_to_t h0.[|p1|].[4*(v j)+1])  (MGroup.int16_to_t h0.[|p2|].[4*(v j)+1])) (MGroup.to_t zeta)); admit()
+  (*assert(v f1 + v f2 <= 2 * params_q /\ v f1 + v f2 >= - 2 * params_q);
+  assert_norm( 2 * params_q < pow2 15);
+  assert(range (v f1 + v f2) S16);
+  MGroup.plus_lemma_int16 f1 f2 (f1 +! f2);
+  assert(MGroup.int16_to_t (f1+!f2) == Group.plus_t (MGroup.to_t f1) (MGroup.to_t f2));
+  assert(MGroup.int16_to_t (f1+!f2) == Group.plus_t (Group.mul_t (MGroup.int16_to_t h0.[|p1|].[4*(v j)]) (MGroup.int16_to_t h0.[|p2|].[4*(v j)])) (Group.mul_t (Group.mul_t (MGroup.int16_to_t h0.[|p1|].[4*(v j)+1]) (MGroup.int16_to_t h0.[|p2|].[4*(v j)+1])) (MGroup.to_t zeta)));
+  assert(MGroup.int16_to_t (f1+!f2) == Group.plus_t (Group.mul_t (MGroup.int16_to_t h0.[|p1|].[4*(v j)]) (MGroup.int16_to_t h0.[|p2|].[4*(v j)])) (Group.mul_t (Group.mul_t (MGroup.int16_to_t h0.[|p1|].[4*(v j)+1]) (MGroup.int16_to_t h0.[|p2|].[4*(v j)+1])) (Lib.Arithmetic.Ring.exp #Group.t #Spec.Kyber2.Ring.ring_t (Spec.Kyber2.Group.mk_t params_zeta) (2*(Lib.Arithmetic.Sums.br 7 (2*(v j))) +1))));
+  FStar.Math.Lemmas.cancel_mul_div (2*(v j)) 2;
+  FStar.Math.Lemmas.swap_mul (2*(v j)) 2;
+  FStar.Math.Lemmas.paren_mul_right 2 2 (v j);
+  assert(2 * (2* v j) == 4 * v j);
+  assert((4*(v j)) / 2 == 2*(v j));
+  assert(MGroup.int16_to_t (f1+!f2) == Group.plus_t (Group.mul_t (MGroup.int16_to_t h0.[|p1|].[4*(v j)]) (MGroup.int16_to_t h0.[|p2|].[4*(v j)])) (Group.mul_t (Group.mul_t (MGroup.int16_to_t h0.[|p1|].[4*(v j)+1]) (MGroup.int16_to_t h0.[|p2|].[4*(v j)+1])) (Lib.Arithmetic.Ring.exp #Group.t #Spec.Kyber2.Ring.ring_t (Spec.Kyber2.Group.mk_t params_zeta) (2*(Lib.Arithmetic.Sums.br 7 ((4*(v j))/2)) +1))));
+  Lib.Poly.NTT2.lib_ntt_mul_even_lemma_instantiate 7 (Spec.Kyber2.Group.mk_t params_zeta) (Seq.map MGroup.int16_to_t h0.[|p1|]) (Seq.map MGroup.int16_to_t h0.[|p2|]) (Lib.Poly.NTT2.lib_ntt_mul #Group.t #Spec.Kyber2.Ring.ring_t #params_n 7 (Spec.Kyber2.Group.mk_t params_zeta) (Seq.map MGroup.int16_to_t h0.[|p1|]) (Seq.map MGroup.int16_to_t h0.[|p2|])) (4*(v j));
+  assert(MGroup.int16_to_t (f1+!f2) == (Lib.Poly.NTT2.lib_ntt_mul #Group.t #Spec.Kyber2.Ring.ring_t #params_n 7 (Spec.Kyber2.Group.mk_t params_zeta) (Seq.map MGroup.int16_to_t h0.[|p1|]) (Seq.map MGroup.int16_to_t h0.[|p2|])).[4*(v j)]);
+  output.(4ul*!j) <- f1 +! f2
