code/kyber2/impl/Impl.Kyber2.Kem.fst
@@ -1,0 +1,128 @@
+module Impl.Kyber2.Kem
+
+open Impl.Kyber2.Indcpa
+
+open FStar.Mul
+
+open Spec.Kyber2.Params
+open Spec.Powtwo.Lemmas
+open Lib.Poly
+open Lib.Poly.NTT2
+open Lib.NumericTypes
+
+open Lib.Arithmetic.Group
+open Lib.Arithmetic.Ring
+open Lib.Arithmetic.Sums
+open Lib.Arithmetic.Group.Uint_t
+open Lib.Arithmetic.Ring.Uint_t
+
+open Lib.Sequence
+open Lib.ByteSequence
+open Lib.IntTypes
+open Lib.NumericTypes
+
+open Lib.ModularArithmetic
+open Lib.ModularArithmetic.Lemmas
+
+open Impl.Kyber2.FunctionInstantiation
+open Impl.Kyber2.CBD
+
+open FStar.Math.Lemmas
+
+module Seq = Lib.Sequence
+module Buf = Lib.Buffer
+
+let sklen:size_t = size Spec.Kyber2.Kem.sklen
+let pklen:size_t = size Spec.Kyber2.Kem.pklen
+let ciphertextlen = size Spec.Kyber2.Kem.ciphertextlen
+
+val keygen:
+  coins: lbuffer uint8 32ul
+  -> indcpacoins:lbuffer uint8 32ul
+  -> pk:lbuffer uint8 pklen
+  -> sk:lbuffer uint8 sklen
+  -> Stack bool
+    (requires fun h -> live h coins /\ live h indcpacoins /\ live h pk /\ live h sk /\
+                    Buf.disjoint coins indcpacoins /\ Buf.disjoint coins pk /\ Buf.disjoint coins sk /\
+                    Buf.disjoint indcpacoins pk /\ Buf.disjoint indcpacoins sk /\
+                    Buf.disjoint pk sk)
+    (ensures fun h0 b h1 -> modifies2 pk sk h0 h1 /\ match Spec.Kyber2.Kem.keygen h0.[|coins|] h0.[|indcpacoins|] with
+      |None -> b == false
+      |Some (p, s) -> b == true /\ h1.[|pk|] == p /\ h1.[|sk|] == s)
+
+let keygen coins indcpacoins pk sk =
+  push_frame ();
+  let b = keygen indcpacoins coins pk (Buf.sub sk 0ul Impl.Kyber2.Indcpa.sklen) in
+  if (b == true) then
+    (Buf.copy (Buf.sub sk Impl.Kyber2.Indcpa.sklen pklen) pk;
+     hash_h pklen pk (Buf.sub sk (Impl.Kyber2.Indcpa.sklen+!pklen) 32ul);
+     Buf.copy (Buf.sub sk (Impl.Kyber2.Indcpa.sklen+!pklen+!32ul) 32ul) coins);
+  pop_frame ();
+  admit();
+  b
+
+val enc:
+  pk:lbuffer uint8 pklen
+  -> msgcoins:lbuffer uint8 32ul
+  -> sharedkeylen:size_t
+  -> ciphertext:lbuffer uint8 ciphertextlen
+  -> sharedkey:lbuffer uint8 sharedkeylen
+  -> Stack bool
+    (requires fun h -> live h pk /\ live h msgcoins /\ live h ciphertext /\ live h sharedkey /\
+                    Buf.disjoint pk msgcoins /\ Buf.disjoint pk ciphertext /\ Buf.disjoint pk sharedkey /\
+                    Buf.disjoint msgcoins ciphertext /\ Buf.disjoint msgcoins ciphertext /\
+                    Buf.disjoint ciphertext sharedkey)
+    (ensures fun h0 b h1 -> modifies2 ciphertext sharedkey h0 h1 /\ match Spec.Kyber2.Kem.enc h0.[|pk|] h0.[|msgcoins|] (v sharedkeylen) with
+      |None -> b == false
+      |Some (c,k) -> b == true /\ h1.[|ciphertext|] == c /\ h1.[|sharedkey|] == k)
+
+let enc pk msgcoins sharedkeylen ciphertext sharedkey =
+  push_frame ()
+  let m = Buf.create 64ul 0ul in
+  let r = Buf.create 32ul 0ul in
+  let kbar = Buf.create 64ul 0ul in
+  hash_h 32ul msgcoins (Buf.sub m 0ul 32ul);
+  hash_h pklen pk (Buf.sub m 32ul 32ul);
+  hash_g 64ul m (Buf.sub kbar 0ul 32ul) r;
+  let b = enc pk (Buf.sub m 0ul 32ul) r ciphertext in
+  if (b==true) then
+    (hash_h ciphertextlen ciphertext (Buf.sub kbar 32ul 32ul);
+    kdf 64ul sharedkeylen kbar sharedkey);
+  pop_frame ();
+  admit();
+  b
+
+val dec:
+  ciphertext:lbuffer uint8 ciphertextlen
+  -> sk:lbuffer uint8 sklen
+  -> sharedkeylen:size_t
+  -> sharedkey:lbuffer uint8 sharedkeylen
+  -> Stack unit
+    (requires fun h -> live h ciphertext /\ live h sk /\ live h sharedkey /\
+                    Buf.disjoint ciphertext sk /\ Buf.disjoint ciphertext sharedkey /\
+                    Buf.disjoint sk sharedkey)
+    (ensures fun h0 _ h1 -> modifies1 sharedkey h0 h1 /\ h1.[|sharedkey|] == Spec.Kyber2.Kem.dec h0.[|ciphertext|] h0.[|sk|] (v sharedkeylen))
+
+let dec ciphertext sk sharedkeylen sharedkey =
+  push_frame ();
+  let sk' = Buf.sub sk 0ul Indcpa.sklen in
+  let pk' = Buf.sub sk Indcpa.sklen Indcpa.pklen in
+  let h = Buf.sub sk (Indcpa.sklen+!Indcpa.pklen) 32ul in
+  let z = Seq.sub sk (Indcpa.sklen+!Indcpa.pklen+!32ul) 32ul in
+  let m' = Buf.create 64ul 0ul in
+  let kbar' = Buf.create 64ul 0ul in
+  let r' = Buf.create 32ul 0ul in
+  let c' = Buf.create Indcpa.ciphertextlen 0ul in
+  dec sk' ciphertext m';
+  Buf.copy (Buf.sub m' 32ul 32ul) h;
+  hash_g 64ul m';
+  let b = Indcpa.enc pk' m' r' c' in
+  hash_h ciphertextlen c (Buf.sub kbar' 32ul 32ul);
+  if (b==true && Lib.ByteBuffer.lbytes_eq ciphertext c') then
+    kdf 64ul sharedkeylen kbar' sharedkey
+  else (
+    Buf.copy (Buf.sub kbar' 0ul 32ul) z;
+    kdf 64ul sharedkeylen kbar' sharedkey
+  );
+  admit();
+  pop_frame ()
