code/kyber2/impl/Impl.Kyber2.NTT.fsti
@@ -1,0 +1,37 @@
+module Impl.Kyber2.NTT
+
+open FStar.HyperStack
+open FStar.HyperStack.ST
+open FStar.Mul
+
+open Impl.Kyber2.Group
+open Impl.Kyber2.Ring
+open Lib.Sequence
+open Lib.Buffer
+
+module ST = FStar.HyperStack.ST
+module Buf = Lib.Buffer
+module Seq = Lib.Sequence
+
+open Spec.Kyber2.Params
+open Impl.Kyber2.NumericTypes.MontgomeryInt16
+open Lib.Arithmetic.Sums
+module MGroup = Impl.Kyber2.GroupMontgomery
+module Group = Impl.Kyber2.Group
+
+open FStar.Math.Lemmas
+open Lib.IntTypes
+
+open Spec.Kyber2.NTT
+
+assume val ntt:
+  p:poly
+  -> Stack unit
+    (requires fun h -> live h p /\ (forall (x:size_nat{x<params_n}). v h.[|p|].[x] <= params_q /\ v h.[|p|].[x] >= - params_q)
+    (ensures fun h0 _ h1 -> to_spec_poly h1 p == Spec.Kyber2.NTT.ntt (to_spec_poly h0 p))
+
+assume val nttinv:
+  p:poly
+  -> Stack unit
+    (requires fun h -> live h p /\ (forall (x:size_nat{x<params_n}). v h.[|p|].[x] <= params_q /\ v h.[|p|].[x] >= - params_q)
+    (ensures fun h0 _ h1 -> to_spec_poly h1 p == Spec.Kyber2.NTT.nttinv (to_spec_poly h0 p))
