code/kyber2/impl/Impl.Kyber2.Poly.fst
@@ -1,1 +1,53 @@
 module Impl.Kyber2.Poly
+
+open Spec.Kyber2.Params
+
+open Impl.Kyber2.NumericTypes.MontgomeryInt16
+
+open Lib.Arithmetic.Group
+open Lib.Arithmetic.Ring
+open Lib.Arithmetic.Sums
+open Impl.Kyber2.GroupMontgomery
+open Spec.Kyber2.Reduce
+
+open Lib.Sequence
+open Lib.ByteSequence
+open Lib.IntTypes
+open Lib.NumericTypes
+
+open Lib.ModularArithmetic
+open Lib.ModularArithmetic.Lemmas
+
+open Impl.Kyber2.FunctionInstantiation
+open Impl.Kyber2.CBD
+
+open FStar.Math.Lemmas
+
+open Spec.Kyber2.Poly
+
+module Buf = Lib.Buffer
+module Seq = Lib.Sequence
+
+assume val poly_compress: d:size_t{v d < 16 /\ pow2 (v d) < params_q}
+ -> p:poly
+ -> Stack unit
+   (requires fun h -> live h p)
+   (ensures fun h0 _ h1 -> modifies1 p h0 h1 /\ to_spec_poly h1 p == Spec.Kyber2.Poly.poly_compress (v d) (to_spec_poly h0 p))
+
+assume val poly_decompress: d:size_t{v d < 16 /\ pow2 (v d) < params_q}
+  -> p:poly
+  -> Stack unit
+    (requires fun h -> live h p /\ let sp = to_spec_poly h p in (forall (i:nat). {:pattern (index #_ #params_n sp i)} i < params_n ==> sint_v #S16 #SEC (index #_ #params_n sp i) < pow2 d))
+    (ensures fun h -> modifies1 p h0 h1 /\ to_spec_poly h1 p == Spec.Kyber2.Poly.poly_decompress (v d) (to_spec_poly h0 p))
+
+assume val vec_compress: d:size_t{v d < 16 /\ pow2 (v d) < params_q}
+  -> v0:vec
+  -> Stack unit
+    (requires fun h -> live h v0)
+    (ensures fun h0 _ h1 -> modifies1 v0 h0 h1 /\ to_spec_vec h1 v0 == Spec.Kyber2.Poly.vec_compress (v d) (to_spec_vec h0 v0))
+
+assume val vec_decompress: d:size_t{v d < 16 /\ pow2 (v d) < params_q}
+  -> v0:vec
+  -> Stack unit
+    (requires fun h -> live h v0 /\ let sv = to_spec_vec h v0 in (forall (i:nat{i<params_k}). forall (j:nat{j<params_n}). sint_v #S16 #SEC (index #_ #params_n (index #_ #params_k sv i) j) < pow2 d))
+    (ensures fun h0 _ h1 -> modifies1 v0 h0 h1 /\ to_spec_vec h1 v0 == Spec.Kyber2.Poly.vec_compress (v d) (to_spec_vec h0 v0))
