code/kyber2/README.md
@@ -1,0 +1,6 @@
+folder spec contains a complete and runnable spec for kyber
+
+folder LowSpec contains the same specification than spec, with machine integers
+
+folder impl contains an implementation for kyber as well as a rewritten low level
+specification (same behavior than in spec) to easy the proof of correspondancy between the impl and the spec
