code/kyber2/impl/README.md
@@ -1,0 +1,47 @@
+Library details (files Lib.*) :
+- Arithmetic.Group : declaration of the monoid and group typeclasses, and some type dependant functions acting on them + instances on pure int and nat
+- Arithmetic.Group.Sequence : instances of the above typeclasses on lseq
+- Arithmetic.Group.Uint_t : instances on unsigned machine integer
+- Arithmetic.Ring : the ring typeclass + type dependant functions
+- Arithmetic.Ring.Sequence : ring instance on lseq
+- Arithmetic.Ring.Uint_t : ring instance on unsigned machine integer
+- Arithmetic.Sums : expressing big sums (indexed by n) with lseq and typeclasses + fubini theorem + explicit bit reversal reordering
+- Arithmetic.SumsBuffer : a naive implementation of Sums with buffers
+- Lib.ModularArithmetic : a pure specification of Zq
+- Lib.ModularArithmetic.Lemmas : useful lemmas on Zq arithmetic
+- NumericTypes : recursive declaration of algebraic types : integers of Zq, polynomials, vectors, matrices.
+- Lib.Poly : declaration of addition and multiplication in Zq[X]/(X^n+1) in the normal domain
+- Lib.Poly.NTT : declaration of the NTT used in Kyber Round1 + some properties
+- Lib.Poly.NTT2 : declaration of the NTT used in Kyber Round2 + some properties
+
+Specification details (files Spec.* ) :
+- CBD : the primitives to generate a centered binomial random distribution
+- FunctionInstantiation : the implementation of Kyber's hash functions and key derivation function, as well as a function to generate a uniform distribution on Zq from a random distribution on uint16.
+- Group : declaration of the group arithmetic on Zq with q = 3329 (Kyber spec) using machine integers + constant time operations
+- GroupMontgomery : the group arithmetic on Zq expressed in the montgomery domain
+- Indcpa : the Primitives for the Indcpa scheme + encoding of secrets as byte streams
+- Kem : the CCA-KEM
+- Lemmas : some small lemmas : we should aim to remove this file and integrate those lemmas in other modules
+- NTT : Kyber's mathematical NTT + the induction property satisfied by the NTT
+- NumericTypes : types for Kybers algebraic objects + accessors and modifiers
+- Params : the set of parameters
+- Poly : compression and decompression functions + proof of small error
+- Reduce : montgomery, barrett reduction + division by q=3329 in constant time
+- Ring : the ring Zq in Kyber
+- Unsafe (fsti only) : do not use unless you want to "fill the blanks" with unchecked code. You will need to provide an external implementation during the compilation
+
+Implementation details (files Impl.*) :
+- Sums : implementation of Lib.Sums in the normal integer representation and the montgomery space
+- CBD : implementation of CBD
+- FunctionInstantiation : implementation of hash function, key derivation + random distribution on Zq (normal space + montgomery)
+- Group : implementation of Group in the normal representation
+- GroupMontgomery : in the montgomery space (+ links to and from the normal space)
+- Indcpa : the implementation of the Indcpa scheme (TODO)
+- Kem : the CCA-KEM (TODO)
+- NTT : an attempt to implement NTT with Cooley-Tukey algorithm. if this is not a priority, just use Lib.SumBuffer to build a quadratic implementation (TO FINISH)
+- NumericTypes : the flat implementation of Kyber types as buffers + accessors + modifiers + ghost interpretation as specification types + generators
+- NumericTypes.Montgomery : same as before, but in the montgomery space with systematic modular reductions
+- NumericTypes.MontgomeryInt16 : same as before, but only performs modular reduction when there may be an overflow
+- Poly : implementation of compression and decompression (TODO, mainly map functions)
+- Reduce : the reductions
+- Ring : implementation of Zq ring
